Legrendree
$$n = 0$$
$$ x_ 0=0;C_0=\int_{-1}^{1}1dx = 2$$

$$n = 1$$
$$ x_ 0=- \frac{\sqrt{3}}{3};C_0=\int_{-1}^{1}- \frac{\sqrt{3} \left(x - \frac{\sqrt{3}}{3}\right)}{2}dx = 1$$
$$ x_ 1=\frac{\sqrt{3}}{3};C_1=\int_{-1}^{1}\frac{\sqrt{3} \left(x + \frac{\sqrt{3}}{3}\right)}{2}dx = 1$$

$$n = 2$$
$$ x_ 0=0;C_0=\int_{-1}^{1}- \frac{5 \left(x - \frac{\sqrt{15}}{5}\right) \left(x + \frac{\sqrt{15}}{5}\right)}{3}dx = \frac{8}{9}$$
$$ x_ 1=- \frac{\sqrt{15}}{5};C_1=\int_{-1}^{1}\frac{5 x \left(x - \frac{\sqrt{15}}{5}\right)}{6}dx = \frac{5}{9}$$
$$ x_ 2=\frac{\sqrt{15}}{5};C_2=\int_{-1}^{1}\frac{5 x \left(x + \frac{\sqrt{15}}{5}\right)}{6}dx = \frac{5}{9}$$

$$n = 3$$
$$ x_ 0=- \sqrt{\frac{3}{7} - \frac{2 \sqrt{30}}{35}};C_0=\int_{-1}^{1}- \frac{\left(x - \sqrt{\frac{3}{7} - \frac{2 \sqrt{30}}{35}}\right) \left(x - \sqrt{\frac{2 \sqrt{30}}{35} + \frac{3}{7}}\right) \left(x + \sqrt{\frac{2 \sqrt{30}}{35} + \frac{3}{7}}\right)}{2 \sqrt{\frac{3}{7} - \frac{2 \sqrt{30}}{35}} \left(- \sqrt{\frac{3}{7} - \frac{2 \sqrt{30}}{35}} + \sqrt{\frac{2 \sqrt{30}}{35} + \frac{3}{7}}\right) \left(- \sqrt{\frac{2 \sqrt{30}}{35} + \frac{3}{7}} - \sqrt{\frac{3}{7} - \frac{2 \sqrt{30}}{35}}\right)}dx = \frac{\sqrt{30}}{36} + \frac{1}{2}$$
$$ x_ 1=\sqrt{\frac{3}{7} - \frac{2 \sqrt{30}}{35}};C_1=\int_{-1}^{1}\frac{\left(x + \sqrt{\frac{3}{7} - \frac{2 \sqrt{30}}{35}}\right) \left(x - \sqrt{\frac{2 \sqrt{30}}{35} + \frac{3}{7}}\right) \left(x + \sqrt{\frac{2 \sqrt{30}}{35} + \frac{3}{7}}\right)}{2 \sqrt{\frac{3}{7} - \frac{2 \sqrt{30}}{35}} \left(\sqrt{\frac{3}{7} - \frac{2 \sqrt{30}}{35}} + \sqrt{\frac{2 \sqrt{30}}{35} + \frac{3}{7}}\right) \left(- \sqrt{\frac{2 \sqrt{30}}{35} + \frac{3}{7}} + \sqrt{\frac{3}{7} - \frac{2 \sqrt{30}}{35}}\right)}dx = \frac{\sqrt{30}}{36} + \frac{1}{2}$$
$$ x_ 2=- \sqrt{\frac{2 \sqrt{30}}{35} + \frac{3}{7}};C_2=\int_{-1}^{1}- \frac{\left(x - \sqrt{\frac{3}{7} - \frac{2 \sqrt{30}}{35}}\right) \left(x + \sqrt{\frac{3}{7} - \frac{2 \sqrt{30}}{35}}\right) \left(x - \sqrt{\frac{2 \sqrt{30}}{35} + \frac{3}{7}}\right)}{2 \sqrt{\frac{2 \sqrt{30}}{35} + \frac{3}{7}} \left(- \sqrt{\frac{2 \sqrt{30}}{35} + \frac{3}{7}} - \sqrt{\frac{3}{7} - \frac{2 \sqrt{30}}{35}}\right) \left(- \sqrt{\frac{2 \sqrt{30}}{35} + \frac{3}{7}} + \sqrt{\frac{3}{7} - \frac{2 \sqrt{30}}{35}}\right)}dx = \frac{1}{2} - \frac{\sqrt{30}}{36}$$
$$ x_ 3=\sqrt{\frac{2 \sqrt{30}}{35} + \frac{3}{7}};C_3=\int_{-1}^{1}\frac{\left(x - \sqrt{\frac{3}{7} - \frac{2 \sqrt{30}}{35}}\right) \left(x + \sqrt{\frac{3}{7} - \frac{2 \sqrt{30}}{35}}\right) \left(x + \sqrt{\frac{2 \sqrt{30}}{35} + \frac{3}{7}}\right)}{2 \sqrt{\frac{2 \sqrt{30}}{35} + \frac{3}{7}} \left(- \sqrt{\frac{3}{7} - \frac{2 \sqrt{30}}{35}} + \sqrt{\frac{2 \sqrt{30}}{35} + \frac{3}{7}}\right) \left(\sqrt{\frac{3}{7} - \frac{2 \sqrt{30}}{35}} + \sqrt{\frac{2 \sqrt{30}}{35} + \frac{3}{7}}\right)}dx = \frac{1}{2} - \frac{\sqrt{30}}{36}$$

$$n = 4$$
$$ x_ 0=0;C_0=\int_{-1}^{1}\frac{\left(x - \sqrt{\frac{5}{9} - \frac{2 \sqrt{70}}{63}}\right) \left(x + \sqrt{\frac{5}{9} - \frac{2 \sqrt{70}}{63}}\right) \left(x - \sqrt{\frac{2 \sqrt{70}}{63} + \frac{5}{9}}\right) \left(x + \sqrt{\frac{2 \sqrt{70}}{63} + \frac{5}{9}}\right)}{\left(\frac{5}{9} - \frac{2 \sqrt{70}}{63}\right) \left(\frac{2 \sqrt{70}}{63} + \frac{5}{9}\right)}dx = \frac{128}{225}$$
$$ x_ 1=- \sqrt{\frac{5}{9} - \frac{2 \sqrt{70}}{63}};C_1=\int_{-1}^{1}\frac{x \left(x - \sqrt{\frac{5}{9} - \frac{2 \sqrt{70}}{63}}\right) \left(x - \sqrt{\frac{2 \sqrt{70}}{63} + \frac{5}{9}}\right) \left(x + \sqrt{\frac{2 \sqrt{70}}{63} + \frac{5}{9}}\right)}{2 \cdot \left(\frac{5}{9} - \frac{2 \sqrt{70}}{63}\right) \left(- \sqrt{\frac{5}{9} - \frac{2 \sqrt{70}}{63}} + \sqrt{\frac{2 \sqrt{70}}{63} + \frac{5}{9}}\right) \left(- \sqrt{\frac{2 \sqrt{70}}{63} + \frac{5}{9}} - \sqrt{\frac{5}{9} - \frac{2 \sqrt{70}}{63}}\right)}dx = - \frac{1134}{-800 + 200 \sqrt{70}} + \frac{12 \sqrt{70}}{-160 + 40 \sqrt{70}} + \frac{210}{-160 + 40 \sqrt{70}}$$
$$ x_ 2=\sqrt{\frac{5}{9} - \frac{2 \sqrt{70}}{63}};C_2=\int_{-1}^{1}\frac{x \left(x + \sqrt{\frac{5}{9} - \frac{2 \sqrt{70}}{63}}\right) \left(x - \sqrt{\frac{2 \sqrt{70}}{63} + \frac{5}{9}}\right) \left(x + \sqrt{\frac{2 \sqrt{70}}{63} + \frac{5}{9}}\right)}{2 \cdot \left(\frac{5}{9} - \frac{2 \sqrt{70}}{63}\right) \left(\sqrt{\frac{5}{9} - \frac{2 \sqrt{70}}{63}} + \sqrt{\frac{2 \sqrt{70}}{63} + \frac{5}{9}}\right) \left(- \sqrt{\frac{2 \sqrt{70}}{63} + \frac{5}{9}} + \sqrt{\frac{5}{9} - \frac{2 \sqrt{70}}{63}}\right)}dx = - \frac{1134}{-800 + 200 \sqrt{70}} + \frac{12 \sqrt{70}}{-160 + 40 \sqrt{70}} + \frac{210}{-160 + 40 \sqrt{70}}$$
$$ x_ 3=- \sqrt{\frac{2 \sqrt{70}}{63} + \frac{5}{9}};C_3=\int_{-1}^{1}\frac{x \left(x - \sqrt{\frac{5}{9} - \frac{2 \sqrt{70}}{63}}\right) \left(x + \sqrt{\frac{5}{9} - \frac{2 \sqrt{70}}{63}}\right) \left(x - \sqrt{\frac{2 \sqrt{70}}{63} + \frac{5}{9}}\right)}{2 \cdot \left(\frac{2 \sqrt{70}}{63} + \frac{5}{9}\right) \left(- \sqrt{\frac{2 \sqrt{70}}{63} + \frac{5}{9}} - \sqrt{\frac{5}{9} - \frac{2 \sqrt{70}}{63}}\right) \left(- \sqrt{\frac{2 \sqrt{70}}{63} + \frac{5}{9}} + \sqrt{\frac{5}{9} - \frac{2 \sqrt{70}}{63}}\right)}dx = - \frac{210}{160 + 40 \sqrt{70}} + \frac{12 \sqrt{70}}{160 + 40 \sqrt{70}} + \frac{1134}{800 + 200 \sqrt{70}}$$
$$ x_ 4=\sqrt{\frac{2 \sqrt{70}}{63} + \frac{5}{9}};C_4=\int_{-1}^{1}\frac{x \left(x - \sqrt{\frac{5}{9} - \frac{2 \sqrt{70}}{63}}\right) \left(x + \sqrt{\frac{5}{9} - \frac{2 \sqrt{70}}{63}}\right) \left(x + \sqrt{\frac{2 \sqrt{70}}{63} + \frac{5}{9}}\right)}{2 \cdot \left(\frac{2 \sqrt{70}}{63} + \frac{5}{9}\right) \left(- \sqrt{\frac{5}{9} - \frac{2 \sqrt{70}}{63}} + \sqrt{\frac{2 \sqrt{70}}{63} + \frac{5}{9}}\right) \left(\sqrt{\frac{5}{9} - \frac{2 \sqrt{70}}{63}} + \sqrt{\frac{2 \sqrt{70}}{63} + \frac{5}{9}}\right)}dx = - \frac{210}{160 + 40 \sqrt{70}} + \frac{12 \sqrt{70}}{160 + 40 \sqrt{70}} + \frac{1134}{800 + 200 \sqrt{70}}$$

